code/ecdsa/dist/Hacl_Hash_Definitions.c
@@ -24,6 +24,8 @@
 
 #include "Hacl_Hash_Definitions.h"
 
+
+
 uint32_t Hacl_Hash_Definitions_word_len(Spec_Hash_Definitions_hash_alg a)
 {
   switch (a)
@@ -62,7 +64,7 @@ uint32_t Hacl_Hash_Definitions_word_len(Spec_Hash_Definitions_hash_alg a)
       }
     default:
       {
-        KRML_HOST_EPRINTF("KreMLin incomplete match at %s:%d\n", __FILE__, __LINE__);
+        KRML_HOST_EPRINTF("KaRaMeL incomplete match at %s:%d\n", __FILE__, __LINE__);
         KRML_HOST_EXIT(253U);
       }
   }
@@ -106,7 +108,7 @@ uint32_t Hacl_Hash_Definitions_block_len(Spec_Hash_Definitions_hash_alg a)
       }
     default:
       {
-        KRML_HOST_EPRINTF("KreMLin incomplete match at %s:%d\n", __FILE__, __LINE__);
+        KRML_HOST_EPRINTF("KaRaMeL incomplete match at %s:%d\n", __FILE__, __LINE__);
         KRML_HOST_EXIT(253U);
       }
   }
@@ -150,7 +152,7 @@ uint32_t Hacl_Hash_Definitions_hash_word_len(Spec_Hash_Definitions_hash_alg a)
       }
     default:
       {
-        KRML_HOST_EPRINTF("KreMLin incomplete match at %s:%d\n", __FILE__, __LINE__);
+        KRML_HOST_EPRINTF("KaRaMeL incomplete match at %s:%d\n", __FILE__, __LINE__);
         KRML_HOST_EXIT(253U);
       }
   }
@@ -194,7 +196,7 @@ uint32_t Hacl_Hash_Definitions_hash_len(Spec_Hash_Definitions_hash_alg a)
       }
     default:
       {
-        KRML_HOST_EPRINTF("KreMLin incomplete match at %s:%d\n", __FILE__, __LINE__);
+        KRML_HOST_EPRINTF("KaRaMeL incomplete match at %s:%d\n", __FILE__, __LINE__);
         KRML_HOST_EXIT(253U);
       }
   }
