code/ecdsa/dist/Hacl_Impl_Blake2_Constants.c
@@ -24,6 +24,8 @@
 
 #include "Hacl_Impl_Blake2_Constants.h"
 
+
+
 const
 uint32_t
 Hacl_Impl_Blake2_Constants_sigmaTable[160U] =
