code/ecdsa/Hacl.Impl.EC.Exponent.fsti
@@ -27,7 +27,7 @@ val exponent: #c: curve -> a: felem c -> result: felem c -> tempBuffer: lbuffer 
 
 [@CInline]
 val square_root: #c: curve -> a: felem c -> result: felem c -> Stack unit 
-  (requires fun h -> live h a /\ live h result /\ as_nat c h a < getPrime c)
+  (requires fun h -> live h a /\ live h result /\ as_nat c h a < getPrime c /\ disjoint a result)
   (ensures fun h0 _ h1 -> modifies (loc a |+| loc result) h0 h1 /\
     as_nat c h1 result < getPrime c /\
     fromDomain #c (as_nat c h1 result) = sq_root_spec #c #DH (fromDomain #c (as_nat c h0 a)) /\
